updates

lectures/PulseIntro.fst
@@ -2,6 +2,10 @@ module PulseIntro
 #lang-pulse
 open Pulse
 
+(******************************************************************************)
+(* Section: Pulse Basics *)
+(******************************************************************************)
+
 let fstar_five : int = 5
 
 (*
@@ -59,8 +63,7 @@ Ownership and permission
       `PureIntroSupport.fst`.
 *)
 
-(* UNCOMMENT AND EXPECT FAILURE *)
-(*
+[@@expect_failure]
 fn five' (x : ref int)
   requires emp
   returns n:int
@@ -70,11 +73,18 @@ fn five' (x : ref int)
   x := v + 1;
   fstar_five
 }
-*)
 
 fn incr (x:ref int)
-requires pts_to x 'i
+requires pts_to x 'i (* implicitly bound logical variable *)
 ensures pts_to x ('i + 1)
+{
+    let v = !x;
+    x := v + 1;
+}
+
+fn incr_explicit_i (x:ref int) (i:erased int)
+requires pts_to x i (* explicitly bound logical variable *)
+ensures pts_to x (i + 1)
 {
     let v = !x;
     x := v + 1;
@@ -133,4 +143,460 @@ requires pts_to x 'i ** f
 ensures pts_to x ('i + 1) ** f
 {
    incr x;
+}
+
+(******************************************************************************)
+(* Section: Mutable References *)
+(******************************************************************************)
+
+(*
+
+* Aim to have memory management without GC
+  + Be able to target C or Rust
+* Different kinds of references
+  + Stack, Heap and Ghost
+
+*)
+
+(* [ref t] type is agnostic to whether it is in heap or stack. Comes from
+   [Pulse.Lib.Reference.ref t] *)
+
+fn swap #a (r0 r1:ref a)
+requires pts_to r0 'v0 ** pts_to r1 'v1
+ensures pts_to r0 'v1 ** pts_to r1 'v0
+{
+    let v0 = !r0;
+    let v1 = !r1;
+    r0 := v1;
+    r1 := v0;
+}
+
+(* Reading a reference *)
+
+fn value_of (#a:Type) (r:ref a)
+requires pts_to r 'v
+returns v:a
+ensures pts_to r 'v ** pure (v == 'v)
+{
+    !r;
+}
+
+fn value_of_explicit (#a:Type) (r:ref a) (#w:erased a)
+requires pts_to r w
+returns v:a
+ensures pts_to r w ** pure (v == reveal w)
+{
+    !r;
+}
+
+[@@expect_failure]
+fn value_of_explicit_fail (#a:Type) (r:ref a) (#w:erased a)
+requires pts_to r w
+returns v:a
+ensures pts_to r w ** pure (v == reveal w)
+{
+    reveal w (* cannot use erased values in non-ghost computations *)
+}
+
+(* Writing to a reference *)
+
+fn assign (#a:Type) (r:ref a) (v:a)
+requires pts_to r 'v
+ensures pts_to r v
+{
+    r := v;
+}
+
+fn add (r:ref int) (n:int)
+requires pts_to r 'v
+ensures pts_to r ('v + n)
+{
+    let v = !r;
+    r := v + n;
+}
+
+open FStar.Mul
+
+fn quadruple (r:ref int)
+requires pts_to r 'v
+ensures pts_to r (4 * 'v)
+{
+    let v1 = !r;
+    add r v1;
+    let v2 = !r;
+    add r v2;
+}
+
+(* Pulse type checking has two components)
+   1. Typing environment
+   2. `slprop` context (or context for short)
+
+   If {p ** q} goal {r ** q} holds and {p} goal {r} also holds, then we call [p]
+   the "support" of [goal] and [q] the "frame" of [goal].
+*)
+
+[@@expect_failure] //comment this line to see the output of [show_proof_state]
+fn quadruple' (r:ref int)
+requires pts_to r 'v
+ensures pts_to r (4 * 'v)
+{
+    let v1 = !r; // Env=v1:int; _:squash (v1 == 'v)       Ctxt= pts_to r v1
+    add r v1;    // ...                                   Ctxt= pts_to r (v1 + v1)
+    show_proof_state;
+    let v2 = !r; // Env=...; v2:int; _:squash(v2==v1+v1)  Ctxt= pts_to r v2
+    add r v2;    // Env=...                               Ctxt= pts_to r (v2 + v2)
+                 // ..                                    Ctxt= pts_to r (4 * 'v)
+    show_proof_state;
+
+}
+
+[@@expect_failure] //Stateful commands are explicitly sequenced
+fn quad_fail (r:ref int)
+requires pts_to r 'v
+ensures pts_to r (4 * 'v)
+{
+    add r (!r);
+    add r (!r);
+}
+
+(* Fractional Permissions *)
+
+(* Actual type of [pts_to]) is:
+
+   val pts_to (#a:Type u#0) (r:ref a) (#p:perm) (v:a) : vprop
+
+  The [perm] argument is interesting.
+  * 1.0R default
+  * 0.0R < p <= 1.0R
+  * Write requires 1.0R
+  * Read can be done at any value of perm.
+*)
+
+fn assign_full_perm (#a:Type) (r:ref a) (v:a)
+requires pts_to r #1.0R 'v
+ensures pts_to r #1.0R v
+{
+    r := v;
+}
+
+fn value_of_perm #a #p (r:ref a)
+requires pts_to r #p 'v
+returns v:a
+ensures pts_to r #p 'v ** pure (v == 'v)
+{
+    !r;
+}
+
+#push-options "--print_implicits"
+[@@expect_failure]
+fn assign_perm #a #p (r:ref a) (v:a) (#w:erased a)
+requires pts_to r #p w
+ensures pts_to r #p w
+{
+    r := v;
+}
+#pop-options
+
+fn share_ref #a #p (r:ref a)
+requires pts_to r #p 'v
+ensures pts_to r #(p /. 2.0R) 'v ** pts_to r #(p /. 2.0R) 'v
+{
+    share r;
+}
+
+fn gather_ref #a (#p:perm) (r:ref a)
+requires
+    pts_to r #(p /. 2.0R) 'v0 **
+    pts_to r #(p /. 2.0R) 'v1
+ensures
+    pts_to r #p 'v0 **
+    pure ('v0 == 'v1) //pointed-to witnesses are equal
+{
+    gather r
+}
+
+(* [let mut] creates a new stack ref *)
+fn one ()
+requires emp
+returns v:int
+ensures pure (v == 1)
+{
+                   //     .     |- emp
+    let mut i = 0; // i:ref int |- pts_to i 0
+    incr i;        // i:ref int |- pts_to i (0 + 1)
+    !i             //      .    |- v:int. emp ** pure (v == 1)
+}
+
+[@@expect_failure]
+fn refs_are_scoped ()
+requires emp
+returns s:ref int
+ensures pts_to s 0
+{
+    let mut s = 0;
+    s
+}
+
+module Box = Pulse.Lib.Box
+(* For heap references. Like Rust's Box<T>. Box has the functions pts_to, (!),
+   (:=), share, gather, alloc and free. *)
+
+fn new_heap_ref (#a:Type) (v:a)
+requires emp
+returns r:Box.box a
+ensures Box.pts_to r v
+{
+    Box.alloc v
+}
+
+fn last_value_of #a (r:Box.box a)
+requires Box.pts_to r 'v
+returns v:a
+ensures pure (v == 'v)
+{
+    open Box;
+    let v = !r;
+    free r;
+    v
+}
+
+(* [box t] references can be demoted to regular [ref t] references for code
+   reuse. *)
+fn incr_box (r:Box.box int)
+requires Box.pts_to r 'v
+ensures Box.pts_to r ('v + 1)
+{
+    Box.to_ref_pts_to r;     //pts_to (box_to_ref r) 'v
+    incr (Box.box_to_ref r); //pts_to (box_to_ref r) ('v + 1)
+    Box.to_box_pts_to r      //Box.pts_to r ('v + 1)
+}
+
+(******************************************************************************)
+(* Section: Existential quantification *)
+(******************************************************************************)
+
+(* Examples: [exists*] is an [slprop -> slprop] constructor.
+
+- exists* (v:nat). pts_to x v
+- exists* v. pts_to x v
+- exists* v1 v2. pts_to x v1 ** pts_to y v2
+
+*)
+
+fn assign2 (#a:Type) (r:ref a) (v:a)
+requires pts_to r 'v //why bother binding this?
+ensures pts_to r v
+{
+    r := v;
+}
+
+fn assign2' #a (x:ref a) (v:a)
+requires
+  exists* w. pts_to x w
+ensures
+  pts_to x v
+{
+  x := v
+}
+
+[@@expect_failure]
+fn incr #a (x:ref int)
+requires
+  exists* w0. pts_to x w
+ensures
+  pts_to x (w0 + 1) //w0 is not in scope here
+{
+  let w = !x
+  x := w + 1
+}
+
+(* Existential quantification often appears in postconditions, e.g., in order to
+   abstract the behavior of function by underspecifying it. *)
+
+fn make_even (x:ref int)
+requires
+  exists* w0. pts_to x w0
+ensures
+  exists* w1. pts_to x w1 ** pure (w1 % 2 == 0)
+{
+  let v = !x;
+  x := v + v;
+}
+
+(* Manipulating existentials
+
+   F* automatically manipulates existentials. But sometimes it is useful to know
+   how to manage them explicitly.
+
+  [with w0...wn. assert p; rest] eliminates existentials when the context
+   contains [exists* x0...xn. p].
+
+   [with] construct binds [w0...wn] to the existentially quantified variables
+   [x0...xn] in the remainder of the scope [rest]. *)
+
+
+fn make_even_explicit (x:ref int)
+requires
+  exists* w0. pts_to x w0
+ensures
+  exists* w1. pts_to x w1 ** pure (w1 % 2 == 0)
+{
+  //show_proof_state;
+  with w0. assert (pts_to x w0);
+  //show_proof_state;
+  let v = !x; // v:int; _:squash(v==w0); Ctxt=pts_to x v
+  x := v + v; //                          ... pts_to x (v + v)
+  //show_proof_state;
+  introduce
+  exists* w1. pts_to x w1 ** pure (w1 % 2 == 0)
+  with (v + v);
+  //show_proof_state;
+}
+
+(* [introduce exists* x1..xn. p with w1..wn] introduces existentials [x1..xn] in
+   the context with witnesses [w1..wn] *)
+
+(* When there is a single existential formula in the context, one can write with
+   [x1..xn. _] to "open" the formula, binding its witnesses in scope. *)
+fn make_even_explicit_alt (x y:ref int)
+requires
+  exists* wx wy. pts_to x wx ** pts_to y wy ** pure (wx % 2 == wy % 2)
+ensures
+  exists* wx' wy'. pts_to x wx' ** pts_to y wy' ** pure (wx' % 2 == 0)
+{
+  //show_proof_state;
+  with wx wy. _;
+  //show_proof_state;
+  let vx = !x;
+  let vy = !y;
+  x := vx + vy;
+  introduce exists* wx' wy'. pts_to x wx' ** pts_to y wy' ** pure (wx' % 2 == 0)
+  with (vx + vy) vy;
+}
+
+
+(******************************************************************************)
+(* Section: User-defined Predicates *)
+(******************************************************************************)
+
+let pts_to_diag
+        #a
+        (r:ref (a & a))
+        (v:a)
+: slprop
+= pts_to r (v, v)
+
+fn double (r:ref (int & int))
+requires pts_to_diag r 'v
+ensures pts_to_diag r (2 * 'v)
+{
+  unfold (pts_to_diag r 'v); //What is [unfold]?
+  let v = !r;
+  let v2 = fst v + snd v;
+  r := (v2, v2);
+  //show_proof_state;
+  fold (pts_to_diag r v2); //What is [fold]?
+}
+
+fn double_alt (r:ref (int & int))
+requires pts_to_diag r 'v
+ensures pts_to_diag r (2 * 'v)
+{
+  unfold pts_to_diag;
+  let v = !r;
+  let v2 = fst v + snd v;
+  r := (v2, v2);
+  fold pts_to_diag;
+}
+
+(* Mutable points *)
+
+noeq
+type point = {
+    x:ref int;
+    y:ref int;
+}
+
+//[is_point] is a "representation predicate" for [point] type.
+let is_point (p:point) (xy: int & int) =
+    pts_to p.x (fst xy) **
+    pts_to p.y (snd xy)
+
+fn move (p:point) (dx:int) (dy:int)
+requires is_point p 'xy
+ensures is_point p (fst 'xy + dx, snd 'xy + dy)
+{
+  unfold is_point;
+  let x = !p.x;
+  let y = !p.y;
+  p.x := x + dx;
+  p.y := y + dy;
+  //show_proof_state;
+  fold (is_point p (x + dx, y + dy));
+    //Pulse cannot infer the instantiation of [is_point] when folding it.
+}
+
+ghost
+fn fold_is_point (p:point)
+requires pts_to p.x 'x ** pts_to p.y 'y
+ensures is_point p (reveal 'x, reveal 'y)
+{
+  fold (is_point p (reveal 'x, reveal 'y))
+}
+
+fn move_alt (p:point) (dx:int) (dy:int)
+requires is_point p 'xy
+ensures is_point p (fst 'xy + dx, snd 'xy + dy)
+{
+  unfold is_point;
+  let x = !p.x;
+  let y = !p.y;
+  p.x := x + dx;
+  p.y := y + dy;
+  fold_is_point p;
+}
+
+(* Rewriting
+
+    with x1 ... xn. rewrite p as q;
+    rest
+
+*)
+
+fn create_and_move ()
+requires emp
+ensures emp
+{
+    let mut x = 0;
+    let mut y = 0;
+    let p = { x; y };
+    //pts_to x 0 ** pts_to y 0
+    with _v. rewrite pts_to x _v as pts_to p.x _v;
+    with _v. rewrite pts_to y _v as pts_to p.y _v;
+    //pts_to p.x 0 ** pts_to p.y 0
+    fold_is_point p;
+    move p 1 1;
+    assert (is_point p (1, 1));
+    unfold is_point;
+    //pts_to p.x (fst (1, 1)) ** pts_to p.y (snd (1, 1))
+    with _v. rewrite pts_to p.x _v as pts_to x _v;
+    with _v. rewrite pts_to p.y _v as pts_to y _v;
+    //pts_to x (fst (1, 1)) ** pts_to y (snd (1, 1))
+}
+
+fn create_and_move_alt ()
+requires emp
+ensures emp
+{
+    let mut x = 0;
+    let mut y = 0;
+    let p = { x; y };
+    rewrite each
+      x as p.x, y as p.y;
+    fold_is_point p;
+    move p 1 1;
+    assert (is_point p (1, 1));
+    unfold is_point;
+    rewrite each
+      p.x as x, p.y as y;
 }
